Fixed mult1_property

Mult.thy
@@ -2,39 +2,27 @@ theory Mult
   imports Add Pred_Logic Inequality
 begin
 
-(*Defining multiplication on N*)
-
 definition mult1 :: "cfunc" where
   "mult1 = (THE v. v: \<nat>\<^sub>c \<rightarrow>  \<nat>\<^sub>c\<^bsup>\<nat>\<^sub>c\<^esup> \<and>
      v \<circ>\<^sub>c zero =  ((zero \<circ>\<^sub>c (right_cart_proj \<nat>\<^sub>c one))\<^sup>\<sharp>) \<and>
-     successor \<circ>\<^sub>c v = (add2  \<circ>\<^sub>c \<langle>(left_cart_proj \<nat>\<^sub>c (\<nat>\<^sub>c\<^bsup>\<nat>\<^sub>c\<^esup>)),(eval_func  \<nat>\<^sub>c \<nat>\<^sub>c) \<rangle>)\<^sup>\<sharp> \<circ>\<^sub>c v)"
+     v \<circ>\<^sub>c successor = (add2  \<circ>\<^sub>c \<langle>(left_cart_proj \<nat>\<^sub>c (\<nat>\<^sub>c\<^bsup>\<nat>\<^sub>c\<^esup>)),(eval_func  \<nat>\<^sub>c \<nat>\<^sub>c) \<rangle>)\<^sup>\<sharp> \<circ>\<^sub>c v)"
 
-(*Need to fix the v below!*)
 lemma mult1_property: "mult1: \<nat>\<^sub>c \<rightarrow>  \<nat>\<^sub>c\<^bsup>\<nat>\<^sub>c\<^esup> \<and>
   mult1 \<circ>\<^sub>c zero =  ((zero \<circ>\<^sub>c (right_cart_proj \<nat>\<^sub>c one))\<^sup>\<sharp>) \<and>
-     successor \<circ>\<^sub>c mult1 = (add2  \<circ>\<^sub>c \<langle>(left_cart_proj \<nat>\<^sub>c (\<nat>\<^sub>c\<^bsup>\<nat>\<^sub>c\<^esup>)),(eval_func  \<nat>\<^sub>c \<nat>\<^sub>c) \<rangle>)\<^sup>\<sharp> \<circ>\<^sub>c mult1"
+     mult1 \<circ>\<^sub>c successor  = (add2  \<circ>\<^sub>c \<langle>(left_cart_proj \<nat>\<^sub>c (\<nat>\<^sub>c\<^bsup>\<nat>\<^sub>c\<^esup>)),(eval_func  \<nat>\<^sub>c \<nat>\<^sub>c) \<rangle>)\<^sup>\<sharp> \<circ>\<^sub>c mult1"
   unfolding mult1_def
-proof (rule theI')
-  have q_type: "((zero \<circ>\<^sub>c (right_cart_proj \<nat>\<^sub>c one))\<^sup>\<sharp>) :  one \<rightarrow>  \<nat>\<^sub>c\<^bsup>\<nat>\<^sub>c\<^esup>"
-    by typecheck_cfuncs
-  have f_type: "((add2  \<circ>\<^sub>c \<langle>(left_cart_proj \<nat>\<^sub>c (\<nat>\<^sub>c\<^bsup>\<nat>\<^sub>c\<^esup>)),(eval_func  \<nat>\<^sub>c \<nat>\<^sub>c) \<rangle>)\<^sup>\<sharp>) : (\<nat>\<^sub>c\<^bsup>\<nat>\<^sub>c\<^esup>) \<rightarrow> (\<nat>\<^sub>c\<^bsup>\<nat>\<^sub>c\<^esup>)"
-    by typecheck_cfuncs
-  show "\<exists>!x. x : \<nat>\<^sub>c \<rightarrow> \<nat>\<^sub>c\<^bsup>\<nat>\<^sub>c\<^esup> \<and>
-         x \<circ>\<^sub>c zero = (zero \<circ>\<^sub>c right_cart_proj \<nat>\<^sub>c one)\<^sup>\<sharp> \<and>
-         successor \<circ>\<^sub>c x = (add2 \<circ>\<^sub>c \<langle>left_cart_proj \<nat>\<^sub>c (\<nat>\<^sub>c\<^bsup>\<nat>\<^sub>c\<^esup>),eval_func \<nat>\<^sub>c \<nat>\<^sub>c\<rangle>)\<^sup>\<sharp> \<circ>\<^sub>c x"
-    sorry    
-qed
+  by (rule theI', typecheck_cfuncs, smt (verit, best) natural_number_object_property)
 
 lemma mult1_type[type_rule]: "mult1 : \<nat>\<^sub>c \<rightarrow> \<nat>\<^sub>c\<^bsup>\<nat>\<^sub>c\<^esup>"
   by (simp add: mult1_property)
 
 lemma mult1_0_eq: "mult1 \<circ>\<^sub>c zero = ((zero \<circ>\<^sub>c (right_cart_proj \<nat>\<^sub>c one))\<^sup>\<sharp>)"
-  using mult1_property  by blast
+  by (simp add: mult1_property)
 
 lemma mult1_comp_succ_eq: "mult1 \<circ>\<^sub>c successor =
   (add2 \<circ>\<^sub>c \<langle>(left_cart_proj \<nat>\<^sub>c (\<nat>\<^sub>c\<^bsup>\<nat>\<^sub>c\<^esup>)),(eval_func  \<nat>\<^sub>c \<nat>\<^sub>c) \<rangle>)\<^sup>\<sharp> \<circ>\<^sub>c mult1"
-  sorry
-
+  by (simp add: mult1_property)
+ 
 definition mult2 :: "cfunc"
   where "mult2 = eval_func \<nat>\<^sub>c \<nat>\<^sub>c \<circ>\<^sub>c (id \<nat>\<^sub>c \<times>\<^sub>f mult1)"
 
